theories/correctness.v
@@ -1,0 +1,202 @@
+From Stdlib Require Import String ZArith List Lia.
+From Stdlib.Relations Require Import Relation_Operators.
+From stdpp Require Import gmap.
+From iris.heap_lang Require Import lang proofmode notation.
+From iris.heap_lang.lib Require Import array.
+From iris.program_logic Require Import weakestpre.
+From Soulite Require Import ast notation semantics heaplang.
+
+Import heap_lang.
+
+Section correctness.
+Context `{!heapGS Σ}.
+
+Definition sl_terminates (e: sl_expr) (v: sl_val): Prop :=
+    exists σ', rtc sl_step (e, empty_state) (ValExpr v, σ').
+
+Inductive closed_expr (bound: list string): sl_expr -> Prop :=
+| ClosedVal v:
+        closed_expr bound (ValExpr v)
+| ClosedVar name
+    (Hbound: List.In name bound):
+        closed_expr bound <{!name}>
+| ClosedList exprs
+    (Hclosed: Forall (closed_expr bound) exprs):
+        closed_expr bound (ListExpr exprs)
+| ClosedUnary op expr
+    (Hclosed: closed_expr bound expr) :
+        closed_expr bound (UnaryExpr op expr)
+| ClosedBinary op lhs rhs
+    (Hlhs: closed_expr bound lhs)
+    (Hrhs: closed_expr bound rhs):
+        closed_expr bound (BinaryExpr op lhs rhs)
+| ClosedTernary cond if_true if_false
+    (Hcond: closed_expr bound cond)
+    (Htrue: closed_expr bound if_true)
+    (Hfalse: closed_expr bound if_false):
+        closed_expr bound <{if_true <- cond;; if_false}>
+| ClosedCallClosure closure args
+    (Hclosure: closed_expr bound closure)
+    (Hargs: Forall (closed_expr bound) args):
+        closed_expr bound (CallClosureExpr closure args)
+| ClosedDeclare name mut type expr
+    (Hclosed: closed_expr (name :: bound) expr):
+        closed_expr bound (DeclareExpr name mut type expr)
+| ClosedAssign name expr
+    (Hbound: List.In name bound)
+    (Hclosed: closed_expr bound expr):
+        closed_expr bound <{name ,= expr}>
+| ClosedClosure params body
+    (Hclosed: closed_expr (params ++ bound) body):
+        closed_expr bound (ClosureExpr params body)
+| ClosedWhile cond body
+    (Hcond: closed_expr bound cond)
+    (Hbody: closed_expr bound body):
+        closed_expr bound (WhileExpr cond body)
+| ClosedSeqDecl name mut type expr e2
+    (Hexpr: closed_expr bound expr)
+    (Hbody: closed_expr (name :: bound) e2):
+        closed_expr bound (SeqExpr (DeclareExpr name mut type expr) e2)
+| ClosedSeq e1 e2
+    (Hleft: closed_expr bound e1)
+    (Hright: closed_expr bound e2):
+        closed_expr bound <{e1 \n\t e2}>.
+
+Definition closed_program (e: sl_expr): Prop :=
+    closed_expr [] e.
+
+(*
+The current compiler treats mutable declarations as references and assignments as stores.
+SimpleSoulite semantics does not model reference values yet, so for now we restrict to the
+immutable fragment to keep the correspondence statement simple.
+*)
+Inductive pure_expr: sl_expr -> Prop :=
+| PureVal v:
+        pure_expr (ValExpr v)
+| PureVar name:
+        pure_expr <{!name}>
+| PureList exprs
+    (Hpure: Forall pure_expr exprs):
+        pure_expr (ListExpr exprs)
+| PureUnary op expr
+    (Hpure: pure_expr expr):
+        pure_expr (UnaryExpr op expr)
+| PureBinary op lhs rhs
+    (Hlhs: pure_expr lhs)
+    (Hrhs: pure_expr rhs):
+        pure_expr (BinaryExpr op lhs rhs)
+| PureTernary cond if_true if_false
+    (Hcond: pure_expr cond)
+    (Htrue: pure_expr if_true)
+    (Hfalse: pure_expr if_false):
+        pure_expr <{if_true <- cond;; if_false}>
+| PureCallClosure closure args
+    (Hclosure: pure_expr closure)
+    (Hargs: Forall pure_expr args):
+        pure_expr (CallClosureExpr closure args)
+| PureDeclare name type expr
+    (Hpure: pure_expr expr):
+        pure_expr (DeclareExpr name false type expr)
+| PureClosure params body (Hpure: pure_expr body):
+        pure_expr (ClosureExpr params body)
+| PureWhile cond body
+    (Hcond: pure_expr cond)
+    (Hbody: pure_expr body):
+        pure_expr (WhileExpr cond body)
+| PureSeq e1 e2
+    (Hleft: pure_expr e1)
+    (Hright: pure_expr e2):
+        pure_expr <{e1 \n\t e2}>.
+
+Fixpoint string_array_rel (l: loc) (s: string): iProp Σ :=
+    match s with
+    | "" => True%I
+    | String c s' =>
+        l ↦ #c ∗ string_array_rel (l +ₗ 1%Z) s'
+    end.
+
+Lemma compile_str_correct (l: loc) (s: string):
+    l ↦∗ replicate (String.length s) #0 -∗
+    WP (compile_str #l s) {{ _, string_array_rel l s }}.
+Admitted.
+
+Fixpoint lit_rel (lit: sl_lit) (v: val) {struct lit}: iProp Σ :=
+    match lit with
+    | LitBoolean b => ⌜v = #b⌝
+    | LitZ n => ⌜v = #n⌝
+    | LitString s =>
+        if Nat.eqb (String.length s) 0 then ⌜v = NONEV⌝
+        else ∃ l : loc, ⌜v = #l⌝ ∗ string_array_rel l s
+    | LitList lits =>
+        let fix list_rel (lits: list sl_lit) (v: val): iProp Σ :=
+            match lits with
+            | [] => ⌜v = NONEV⌝
+            | lit :: lits' =>
+                ∃ l : loc, ∃ v_head v_tail,
+                ⌜v = #l⌝ ∗ l ↦ PairV v_head v_tail ∗ lit_rel lit v_head ∗ list_rel lits' v_tail
+            end%I
+        in list_rel lits v
+    end%I.
+
+Definition list_rel (lits: list sl_lit) (v: val): iProp Σ :=
+    lit_rel (LitList lits) v.
+
+Definition val_rel (v_s: sl_val) (v_h: val): iProp Σ :=
+    match v_s with
+    | LitVal lit => lit_rel lit v_h
+    | ClosureVal params body =>
+        ⌜v_h = compile_closurev_val params (compile_expr body)⌝
+    end%I.
+
+Definition state_rel (_σ: sl_state): iProp Σ := True%I.
+
+Lemma compile_lit_correct (lit: sl_lit):
+    ⊢ WP (compile_lit lit) {{ v, lit_rel lit v }}.
+Proof.
+induction lit as [b|n|s|lits IHlits] using sl_lit_ind.
+- simpl. wp_pures. done.
+- simpl. wp_pures. done.
+- destruct s as [|c s'].
+    + simpl. wp_pures. done.
+    + simpl.
+        wp_apply (wp_allocN with "[]"); admit.
+        (*
+        { iPureIntro. simpl. lia. }
+        iIntros (l) "Hl".
+        wp_pures.
+        wp_bind (compile_str #l (String c s')).
+        wp_apply (compile_str_correct l (String c s') with "Hl").
+        iIntros (_) "Hstr".
+        wp_pures.
+        iApply wp_value.
+        iExists l. iFrame.
+        *)
+- simpl. admit.
+    (*
+    revert IHlits.
+    induction lits as [|lit lits IH]; iIntros (IHlits).
+    + simpl. wp_pures. iApply wp_value. simpl. done.
+    + inversion IHlits as [|lit' lits' Hlit Hrest]; subst.
+        simpl.
+        wp_bind (compile_lit lit).
+        wp_apply Hlit.
+        iIntros (v_head) "Hhead".
+        wp_bind (compile_list (map compile_lit lits)).
+        wp_apply (IH Hrest).
+        iIntros (v_tail) "Htail".
+        wp_pures.
+        wp_alloc l as "Hl".
+        iApply wp_value.
+        iExists l, v_head, v_tail.
+        iFrame.
+    *)
+Admitted.
+
+Lemma compile_expr_correct (e: sl_expr) (v_s: sl_val):
+    closed_program e ->
+    pure_expr e ->
+    sl_terminates e v_s ->
+    ⊢ WP (compile_expr e) {{ v_h, val_rel v_s v_h }}.
+Admitted.
+
+End correctness.
