theories/readme.md
@@ -1,0 +1,45 @@
+# Soulite Subset Formal Verification
+
+This directory contains Rocq proofs that formally verify SimpleSoulite (a simple subset of Soulite) by compiling it to Iris [heap_lang](https://gitlab.mpi-sws.org/iris/iris) and proving a forward simulation between the small‑step semantics of SimpleSoulite and the weakest precondition semantics of HeapLang.
+
+## Prerequisites
+
+- Linux or WSL2 (macOS/Windows may work but are not tested)
+- [Opam](https://opam.ocaml.org/) 2.0+
+- Rocq 8.19+ and Iris 4.2+ (installed via opam)
+
+## Setup
+
+To run the Rocq files for formal verification, initialize the makefile:
+```bash
+coq_makefile -f _CoqProject -o makefile
+```
+This should generate the following three files:
+- `.makefile.d`
+- `makefile`
+- `makefile.conf`
+
+## Development
+
+To compile all `.v` files:
+```bash
+make
+```
+For VsCode, install the VsRocq extension and set the `vsrocqtop` path to your opam‑installed `rocq` binary.
+
+### Project structure
+
+- `ast.v`, SimpleSoulite abstract syntax and types
+- `notation.v`, custom syntax and notation for SimpleSoulite
+- `semantics.v`, small‑step operational semantics of SimpleSoulite
+- `compiler.v`, compiler from SimpleSoulite to heap_lang
+- `correctness.v`, forward simulation proof
+
+### Notable Syntactic Differences
+
+Due to limitations of using Rocq's notation feature, SimpleSoulite's syntax has deviated from Soulite:
+
+- Variable and function names: `var` -> `!"var"`
+- Ternary condition: `if_true <- cond ; if_false` -> `if_true <- cond ;; if_false`
+- Variable assignment: `var = val` -> `var ,= val`
+- Newlines and tabs need to be typed out: `\n` and `\t`
